MECMAR/spec/Base.v
@@ -1,220 +1,11 @@
 From Coq Require Import ZArith Lia List ListSet Bool.
 From Warblre Require Import Tactics List Result.
+From Warblre Require Export Characters Numeric Coercions Errors.
+
+(** Notations for list operations *)
 
 Import Result.Notations.
 Local Open Scope result_flow.
-
-(* 5.2.5 Mathematical Operations
-   «  Mathematical values: Arbitrary real numbers, used as the default numeric type. »
-   «  When the term integer is used in this specification, it refers to a mathematical 
-      value which is in the set of integers, unless otherwise stated. When the term integral 
-      Number is used in this specification, it refers to a Number value whose mathematical
-      value is in the set of integers. »
-   ... so, that should be a Real? (note that "integers" redirects to the second definition).
-*)
-Definition integer := Z.
-Definition non_neg_integer := nat.
-Definition positive_integer := { n: non_neg_integer | (0 < n)%nat }.
-Definition nat_to_nni (n: nat): non_neg_integer := n.
-Definition positive_to_non_neg (n: positive_integer): non_neg_integer := proj1_sig n.
-Definition positive_to_nat (n: positive_integer): nat := proj1_sig n.
-
-Module NonNegInt.
-  Definition to_positive {F: Type} {_: Result.AssertionError F} (n: non_neg_integer): Result positive_integer F.
-    destruct n eqn:Eq_n.
-    - apply Result.assertion_failed.
-    - refine (Success (exist _ n _)). subst. apply Nat.lt_0_succ.
-  Defined.
-
-  Lemma to_positive_soundness {F: Type} {_: Result.AssertionError F}: forall n p, to_positive n = Success p -> proj1_sig p = n.
-  Proof. intros. destruct n; cbn in *. - Result.assertion_failed_helper. - injection H as <-. reflexivity. Qed.
-
-  Lemma to_positive_completeness {F: Type} {_: Result.AssertionError F}: forall n, 0 < n -> exists p, to_positive n = Success p.
-  Proof. intros. destruct n. - lia. - cbn. eexists. reflexivity. Qed.
-End NonNegInt.
-
-
-(* Nat or Infinity *)
-Module NoI.
-  Inductive non_neg_integer_or_inf :=
-  | N (n: non_neg_integer)
-  | Inf.
-
-  Definition eqb (l r: non_neg_integer_or_inf): bool := match l, r with
-  | N l', N r' => Nat.eqb l' r'
-  | Inf, Inf => true
-  | _, _ => false
-  end.
-
-  Definition add (l r: non_neg_integer_or_inf): non_neg_integer_or_inf := match l, r with
-  | N l', N r' => N (Nat.add l' r')
-  | _, _ => Inf
-  end.
-
-  Definition sub (l: non_neg_integer_or_inf) (r: non_neg_integer): non_neg_integer_or_inf := match l with
-  | N l' => N (Nat.sub l' r)
-  | _=> Inf
-  end.
-
-  Definition leqb (l: non_neg_integer) (r: non_neg_integer_or_inf): bool := match r with
-  | N r' => (l <=? r')%nat
-  | Inf => true
-  end.
-
-  Module Coercions.
-    Coercion NoI.N: non_neg_integer >-> non_neg_integer_or_inf.
-  End Coercions.
-End NoI.
-Notation "'+∞'" := NoI.Inf.
-Export NoI(non_neg_integer_or_inf).
-
-Infix "!=?" := (fun l r => negb (Nat.eqb l r)) (at level 70): nat_scope.
-Infix "<=?" := Nat.leb (at level 70, no associativity): nat_scope.
-Infix ">=?" := (fun l r => Nat.leb r l) (at level 70, no associativity): nat_scope.
-
-Declare Scope NoI_scope.
-Delimit Scope NoI_scope with NoI.
-Infix "=?" := NoI.eqb (at level 70): NoI_scope.
-Infix "+" := NoI.add (at level 50, left associativity): NoI_scope.
-Infix "-" := NoI.sub (at level 50, left associativity): NoI_scope.
-Infix "<=?" := NoI.leqb (at level 70, no associativity): NoI_scope.
-
-Infix "=?" := Z.eqb (at level 70): Z_scope.
-Infix "!=?" := (fun l r => negb (Z.eqb l r)) (at level 70): Z_scope.
-Infix "<?" := Z.ltb (at level 70): Z_scope.
-Infix "<=?" := Z.leb (at level 70): Z_scope.
-Infix ">?" := Z.gtb (at level 70): Z_scope.
-Infix ">=?" := Z.geb (at level 70): Z_scope.
-
-Parameter Character: Type.
-Parameter CodePoint: Type.
-Module Character.
-  Parameter eqs: forall (l r: Character), {l = r} + {l <> r}.
-  Parameter eqb: forall (l r: Character), bool.
-  Definition neqb (l r: Character) := negb (eqb l r).
-
-  Parameter numeric_value: Character -> non_neg_integer.
-  Parameter from_numeric_value: non_neg_integer -> Character.
-  Parameter code_point: Character -> CodePoint.
-
-  Axiom numeric_pseudo_bij: forall c, Character.from_numeric_value (Character.numeric_value c) = c.
-
-  Module Unicode.
-    Parameter case_fold: Character -> Character.
-  End Unicode.
-End Character.
-Module CodePoint.
-    Parameter to_upper_case: CodePoint -> CodePoint.
-    Parameter code_points_to_string: CodePoint -> list Character.
-End CodePoint.
-
-Module Characters.
-  Definition NULL: Character := Character.from_numeric_value 0.
-  Definition BACKSPACE: Character := Character.from_numeric_value 8.
-  Definition CHARACTER_TABULATION: Character := Character.from_numeric_value 9.
-  Definition LINE_FEED: Character := Character.from_numeric_value 10.
-  Definition LINE_TABULATION: Character := Character.from_numeric_value 11.
-  Definition FORM_FEED: Character := Character.from_numeric_value 12.
-  Definition CARRIAGE_RETURN: Character := Character.from_numeric_value 13.
-  Definition HYPHEN_MINUS: Character := Character.from_numeric_value 55.
-End Characters.
-
-Parameter GroupName: Type.
-Module GroupName.
-  Parameter eqs: forall (l r: Character), {l = r} + {l <> r}.
-  Parameter eqb: forall (l r: Character), bool.
-  Definition neqb (l r: Character) := negb (eqb l r).
-End GroupName.
-
-Declare Scope Character_scope.
-Delimit Scope Character_scope with Chr.
-Infix "=?" := Character.eqb (at level 70): Character_scope.
-Infix "!=?" := Character.neqb (at level 70): Character_scope.
-
-Declare Scope GroupName_scope.
-Delimit Scope GroupName_scope with GrName.
-Infix "=?" := GroupName.eqb (at level 70): GroupName_scope.
-Infix "!=?" := GroupName.neqb (at level 70): GroupName_scope.
-
-Module CompileError.
-  (* https://github.com/coq/coq/issues/7424 *)
-  Inductive type: let t := Type in t :=
-  | AssertionFailed.
-End CompileError.
-Notation CompileError := CompileError.type.
-
-Module MatchError.
-  Inductive type :=
-  | OutOfFuel
-  | AssertionFailed.
-End MatchError.
-Notation MatchError := MatchError.type.
-
-#[export]
-Instance compile_assertion_error: Result.AssertionError CompileError := { f := CompileError.AssertionFailed }.
-#[export]
-Instance match_assertion_error: Result.AssertionError MatchError := { f := MatchError.AssertionFailed }.
-Notation compile_assertion_failed := (Failure CompileError.AssertionFailed).
-Notation failure := None (only parsing).
-Notation out_of_fuel := (Failure MatchError.OutOfFuel).
-Notation match_assertion_failed := (Failure MatchError.AssertionFailed).
-
-(*  A CharSet is a mathematical set of characters. In the context of a Unicode pattern, “all characters” means
-    the CharSet containing all code point values; otherwise “all characters” means the CharSet containing all
-    code unit values. *)
-Definition CharSet := list Character.
-
-Module CharSet.
-  Definition empty: CharSet := nil.
-  Definition union (l r: CharSet): CharSet := ListSet.set_union Character.eqs l r.
-  Definition singleton (c: Character): CharSet := c :: nil.
-  Definition size (s: CharSet): nat := List.length s.
-  Definition unique {F: Type} {_: Result.AssertionError F} (s: CharSet): Result Character F :=
-    match s with
-    | c :: nil => Success c
-    | _ => Result.assertion_failed
-    end.
-  Definition remove_all (l r: CharSet): CharSet := ListSet.set_diff Character.eqs l r.
-  Definition exist (s: CharSet) (m: Character -> Result bool MatchError): Result bool MatchError :=
-    List.Exists.exist s m.
-  Definition is_empty (s: CharSet): bool :=
-    match s with
-    | nil => true
-    | _ :: _ => false
-    end.
-  Definition filter {F: Type} {_: Result.AssertionError F} (s: CharSet) (f: Character -> Result bool F): Result CharSet F :=
-    List.Filter.filter s f.
-
-  Definition contains (s: CharSet) (c: Character): bool := ListSet.set_mem Character.eqs c s.
-
-  Definition range (l h: nat): CharSet :=
-    List.map Character.from_numeric_value (List.Range.Nat.Bounds.range l (S h)).
-
-  Parameter all: CharSet.
-  Parameter line_terminators: CharSet.
-  Parameter digits: CharSet.
-  Parameter white_spaces: CharSet.
-  Parameter ascii_word_characters: CharSet.
-End CharSet.
-
-
-(* Module IdSet.
-  Parameter t: Type.
-
-  Parameter empty: t.
-  Parameter union: t -> t -> t.
-  Parameter add: IdentifierName -> t -> t.
-  Parameter fold: forall {T: Type}, (IdentifierName -> T -> T) -> t -> T -> T.
-End IdSet. *)
-
-(* Module DMap.
-  Parameter t: Type -> Type.
-
-  Parameter empty: forall T, t T.
-  Parameter add: forall {T: Type}, IdentifierName -> T -> t T -> t T.
-  Parameter remove: forall {T: Type}, IdentifierName -> t T -> t T.
-  (* Parameter removeAll: forall {T: Type}, t T -> IdSet.t -> t T. *)
-End DMap. *)
 
 Class Indexer (I: Type) := {
   index_using: forall (T F: Type) (_: Result.AssertionError F) (ls: list T) (i: I), Result.Result T F;
@@ -238,20 +29,15 @@ Instance pos_indexer: Indexer positive_integer := {
 #[export]
 Instance int_indexer: Indexer Z := {
   index_using := @List.Indexing.Int.indexing;
-  update_using := fun T F f ls i v => Result.assertion_failed;
+  update_using := fun T F f ls i v => Result.assertion_failed; (* This operation is never used. *)
 }.
 
 Notation "ls '[' i ']'" := (indexing ls i) (at level 98, left associativity).
 Notation "'set' ls '[' i ']' ':=' v 'in' z" := (let! ls: list _ =<< update ls i v in z) (at level 200, ls at level 97, i at level 90, right associativity).
 Notation "'set' ls '[' s '---' e ']' ':=' v 'in' z" := (let! ls: list _ =<< List.Update.Nat.Batch.update v ls (List.Range.Nat.Bounds.range (s - 1) (e - 1)) in z) (at level 200, ls at level 97, s at level 90, e at level 90, right associativity).
 
+(** The is (not) operator *)
+
 Notation "m 'is' p" := (match m with | p => true | _ => false end) (at level 100, p pattern, no associativity).
 Notation "m 'is' 'not' p" := (match m with | p => false | _ => true end) (at level 100, p pattern, no associativity).
-
-Module Coercions.
-  Coercion nat_to_nni: nat >-> non_neg_integer.
-  Coercion positive_to_non_neg: positive_integer >-> non_neg_integer.
-  Coercion positive_to_nat: positive_integer >-> nat.
-  Coercion wrap_result := fun (F: Type) (v: non_neg_integer) => @Success _ F v.
-End Coercions.
 
