MECMAR/spec/ClutterFree.v
@@ -1,4 +1,4 @@
-From Warblre Require Import Result Base Patterns Notation Semantics Correctness Compile.
+From Warblre Require Import Result Base Patterns Notation Semantics Match Compile.
 
 Import Result.Notations.
 Local Open Scope result_flow.
