MECMAR/spec/base/Characters.v
@@ -1,0 +1,82 @@
+From Coq Require Import List ListSet.
+From Warblre Require Import List Result Numeric.
+
+(* Parameter Character: Type.
+Parameter CodePoint: Type. *)
+Module Character.
+  Parameter type: Type.
+  Parameter eqs: forall (l r: type), {l = r} + {l <> r}.
+  Parameter eqb: forall (l r: type), bool.
+  Definition neqb (l r: type) := negb (eqb l r).
+
+  Parameter numeric_value: type -> non_neg_integer.
+  Parameter from_numeric_value: non_neg_integer -> type.
+
+  Axiom numeric_pseudo_bij: forall c, Character.from_numeric_value (Character.numeric_value c) = c.
+
+  Module Unicode.
+    Parameter case_fold: type -> type.
+  End Unicode.
+
+  Definition NULL: type := Character.from_numeric_value 0.
+  Definition BACKSPACE: type := Character.from_numeric_value 8.
+  Definition CHARACTER_TABULATION: type := Character.from_numeric_value 9.
+  Definition LINE_FEED: type := Character.from_numeric_value 10.
+  Definition LINE_TABULATION: type := Character.from_numeric_value 11.
+  Definition FORM_FEED: type := Character.from_numeric_value 12.
+  Definition CARRIAGE_RETURN: type := Character.from_numeric_value 13.
+  Definition HYPHEN_MINUS: type := Character.from_numeric_value 55.
+End Character.
+Notation Character := Character.type.
+
+Module CodePoint.
+  Parameter type: Type.
+  Parameter to_upper_case: type -> type.
+  Parameter code_points_to_string: type -> list Character.
+
+  Parameter from_character: Character -> type.
+End CodePoint.
+Notation CodePoint := CodePoint.type.
+
+Declare Scope Character_scope.
+Delimit Scope Character_scope with Chr.
+Infix "=?" := Character.eqb (at level 70): Character_scope.
+Infix "!=?" := Character.neqb (at level 70): Character_scope.
+
+(*  A CharSet is a mathematical set of characters. In the context of a Unicode pattern, “all characters” means
+    the CharSet containing all code point values; otherwise “all characters” means the CharSet containing all
+    code unit values. *)
+Definition CharSet := list Character.
+
+Module CharSet.
+  Definition empty: CharSet := nil.
+  Definition union (l r: CharSet): CharSet := ListSet.set_union Character.eqs l r.
+  Definition singleton (c: Character): CharSet := c :: nil.
+  Definition size (s: CharSet): nat := List.length s.
+  Definition unique {F: Type} {_: Result.AssertionError F} (s: CharSet): Result Character F :=
+    match s with
+    | c :: nil => Success c
+    | _ => Result.assertion_failed
+    end.
+  Definition remove_all (l r: CharSet): CharSet := ListSet.set_diff Character.eqs l r.
+  Definition exist {F: Type} {_: Result.AssertionError F} (s: CharSet) (m: Character -> Result bool F): Result bool F :=
+    List.Exists.exist s m.
+  Definition is_empty (s: CharSet): bool :=
+    match s with
+    | nil => true
+    | _ :: _ => false
+    end.
+  Definition filter {F: Type} {_: Result.AssertionError F} (s: CharSet) (f: Character -> Result bool F): Result CharSet F :=
+    List.Filter.filter s f.
+
+  Definition contains (s: CharSet) (c: Character): bool := ListSet.set_mem Character.eqs c s.
+
+  Definition range (l h: nat): CharSet :=
+    List.map Character.from_numeric_value (List.Range.Nat.Bounds.range l (S h)).
+
+  Parameter all: CharSet.
+  Parameter line_terminators: CharSet.
+  Parameter digits: CharSet.
+  Parameter white_spaces: CharSet.
+  Parameter ascii_word_characters: CharSet.
+End CharSet.
