MECMAR/spec/base/Errors.v
@@ -1,0 +1,25 @@
+From Warblre Require Import Result.
+
+Module CompileError.
+  (* https://github.com/coq/coq/issues/7424 *)
+  Inductive type: let t := Type in t :=
+  | AssertionFailed.
+End CompileError.
+Notation CompileError := CompileError.type.
+
+Module MatchError.
+  Inductive type :=
+  | OutOfFuel
+  | AssertionFailed.
+End MatchError.
+Notation MatchError := MatchError.type.
+
+#[export]
+Instance compile_assertion_error: Result.AssertionError CompileError := { f := CompileError.AssertionFailed }.
+#[export]
+Instance match_assertion_error: Result.AssertionError MatchError := { f := MatchError.AssertionFailed }.
+
+Notation compile_assertion_failed := (Failure CompileError.AssertionFailed).
+Notation failure := None (only parsing).
+Notation out_of_fuel := (Failure MatchError.OutOfFuel).
+Notation match_assertion_failed := (Failure MatchError.AssertionFailed).
